added support for ifelse?

build.py
@@ -48,7 +48,8 @@ CODE_DIRS = ["arch", "impl", "lib"]
 GEN_DIR = "gen"
 
 
-NL_FILES = {"arch/riscv/vale.i.dfy",
+NL_FILES = {
+    # "arch/riscv/vale.i.dfy",
     "impl/riscv/sub_mod_nl_lemmas.i.dfy",
     # "impl/riscv/sub_mod_lemmas.i.dfy",
     "lib/bv_ops_nl.dfy"}
